Mayor cleaning. Many admits removed from infinit proof

concurrency/compiler/CoreSemantics_sum.v
@@ -43,7 +43,7 @@ Definition state_sum_optionmt {Cs Ct M:Type} (cto: option (Ct * option M)): opti
 Definition lt_op (n: nat) (no:option nat): Prop :=
   match no with
     | None => True
-    | Some n' => n <= n' (* smallest is (Some 0) largest is None*) 
+    | Some n' => n < n' (* smallest is (Some 0) largest is None*) 
   end.
 
 Definition initial_core_sum (no:option nat) (Cs Ct:Type) (M: Type)
@@ -52,8 +52,8 @@ Definition initial_core_sum (no:option nat) (Cs Ct:Type) (M: Type)
   nat -> M -> state_sum Cs Ct -> M -> Values.val -> list Values.val -> Prop :=
   fun (n:nat) m c m' val vals =>
     match c with
-    | SState c => lt_op n no /\ sinitial_core n m c m' val vals
-    | TState c => ~lt_op n no /\ tinitial_core n m c m' val vals
+    | SState c => ~lt_op n no /\ sinitial_core n m c m' val vals
+    | TState c => lt_op n no /\ tinitial_core n m c m' val vals
     end.
 
 Definition sum_func {Cs Ct X:Type} (fs:Cs -> X) (ft:Ct-> X) s:=
