concurrency/compiler/multiple_thread_simulation_proof.v
@@ -46,7 +46,7 @@ Require Import VST.concurrency.lib.pair.
 Require Import VST.concurrency.compiler.inject_virtue.
 Require Import VST.concurrency.compiler.concur_match.
 Require Import VST.concurrency.lib.Coqlib3.
- 
+
 
 Set Nested Proofs Allowed.
 Set Bullet Behavior "Strict Subproofs".
@@ -94,8 +94,9 @@ Section ThreadedSimulation.
       
       Inductive match_state:
         forall n, nth_index ->
-          Values.Val.meminj ->
-          ThreadPool (Some 0)%nat -> Memory.Mem.mem -> ThreadPool (Some n) -> Memory.Mem.mem -> Prop:=
+             Values.Val.meminj ->
+             ThreadPool (Some 0)%nat -> Memory.Mem.mem ->
+             ThreadPool (Some n) -> Memory.Mem.mem -> Prop:=
       | refl_match: forall tp m,
           (* mem_compatible tp m -> *)
           match_state 0 nil (Mem.flat_inj (Mem.nextblock m)) tp m tp m
@@ -141,11 +142,11 @@ Section ThreadedSimulation.
         match_case.
         xomega.
       Qed.
-     
+      
       Local Ltac inv_match0:=
         match goal with
-              H: match_state 0 _ _ _ _ _ _ |- _ =>
-              inversion H; subst_sig; try clear H
+          H: match_state 0 _ _ _ _ _ _ |- _ =>
+          inversion H; subst_sig; try clear H
         end.
       Lemma Forall_cat:
         forall {A B} (f: A -> B -> Prop) a1 a2 b1 b2,
@@ -163,34 +164,41 @@ Section ThreadedSimulation.
       Lemma machine_step_traces:
         forall hb m sge U tr1 st1 m1 U' tr1' st1' m1',
           machine_semantics.machine_step (HybConcSem hb m)
-            sge U tr1 st1 m1 U' tr1' st1' m1'->
+                                         sge U tr1 st1 m1 U' tr1' st1' m1'->
           exists tr_tail, tr1' = tr1 ++ tr_tail /\
-                     forall tr2, machine_semantics.machine_step (HybConcSem hb m)
-                         sge U tr2 st1 m1 U' (tr2 ++ tr_tail) st1' m1'.
+                     forall tr2, machine_semantics.machine_step
+                              (HybConcSem hb m)
+                              sge U tr2 st1 m1 U' (tr2 ++ tr_tail) st1' m1'.
       Admitted.
+      
       Lemma trivial_self_injection:
         forall m : option mem,
-          HybridMachine_simulation_properties
+          simulation_properties_exposed
             (HybConcSem (Some 0)%nat m)
             (HybConcSem (Some 0)%nat m)
             invariant
             mem_compatible
-            (match_state 0).
+            (match_state 0)
+            list_lt.
       Proof.
         simpl; intros.
-        econstructor.
+        unshelve econstructor; [econstructor|].
         - eapply list_lt_wf.
         - intros; normal; eauto.
           + econstructor.
-        - intros; normal.
+        - intros; normal_hyp.
+          assert (inject_incr mu (Mem.flat_inj (Mem.nextblock m1'))).
+            { inv_match0; eapply flat_inj_lt.
+              eapply thread_step_mem_fwd; apply H. }
+          normal.
           + econstructor.
-          + eapply inject_incr_trace; try eassumption.
-            inv_match0; eapply flat_inj_lt.
-            eapply thread_step_mem_fwd; apply H.
+          + eapply inject_incr_trace; try eassumption.  
           + left. exists 0%nat; inv_match0.
             do 2 eexists; split; try reflexivity; eauto.
+          + assumption.
         - intros; inv_match0.
-          eapply machine_step_traces in H; normal; subst; eauto.
+          eapply machine_step_traces in H; normal_hyp; subst.
+          do 5 econstructor; repeat weak_split.
           + econstructor.
           + eapply Forall_cat.
             eapply inject_incr_trace; try eassumption.
@@ -198,15 +206,19 @@ Section ThreadedSimulation.
             eapply machine_step_mem_fwd; eauto.
             eapply machine_step_trace_wf; eapply H2.
           + eapply H2.
+          + specialize (H2 tr2); apply machine_step_mem_fwd in H2.
+            apply flat_inj_lt; eauto.
         - intros; inv_match0; normal; eauto.
-        - intros; inv_match0; reflexivity. 
+        - intros; inv_match0; reflexivity.
+        - reflexivity.
+          
           Unshelve.
           all: eauto.
       Qed.
       
       
       Lemma step_diagram_helper:
-        forall (ord: relation nth_index) tr1 tr2 m U hb cd m1' st1' tge st2 m2, 
+        forall mu (ord: relation nth_index) tr1 tr2 m U hb cd m1' st1' tge st2 m2, 
           (exists (st2' : ThreadPool (Some hb)) (m2' : mem) (cd' : nth_index) 
              (mu' : meminj),
               match_state hb cd' mu' st1' m1' st2' m2' /\
@@ -216,7 +228,8 @@ Section ThreadedSimulation.
                  tge U st2 m2 st2' m2' \/
                machine_semantics_lemmas.thread_step_star
                  (HybConcSem (Some hb) m) 
-                 tge U st2 m2 st2' m2' /\ ord cd' cd))
+                 tge U st2 m2 st2' m2' /\ ord cd' cd) /\
+          inject_incr mu mu')
           <->
           exists (st2' : ThreadPool (Some hb)) (m2' : mem) (cd' : nth_index) 
             (mu' : meminj),
@@ -224,7 +237,8 @@ Section ThreadedSimulation.
             Forall2 (inject_mevent mu') tr1 tr2 /\
             (machine_semantics_lemmas.thread_step_plus
                (HybConcSem (Some hb) m) 
-               tge U st2 m2 st2' m2' \/  m2=m2' /\ st2=st2' /\ ord cd' cd).
+               tge U st2 m2 st2' m2' \/  m2=m2' /\ st2=st2' /\ ord cd' cd) /\
+          inject_incr mu mu'.
       Proof.
         intros.
         split; intros; normal; eauto.
@@ -238,108 +252,141 @@ Section ThreadedSimulation.
       Qed.
       
       Lemma inject_mem_event_interpolation:
-            forall jn jSn ev1 ev3,
-            (inject_mem_event (compose_meminj jn jSn)) ev1 ev3 ->
-            exists ev2,
-              inject_mem_event jn ev1 ev2 /\
-              inject_mem_event jSn ev2 ev3 .
-          Proof.
-            intros.
-            destruct ev1.
-            - inv H.
-          Admitted.
-          Lemma inject_mem_sync_interpolation:
-            forall jn jSn ev1 ev3,
-            (inject_sync_event (compose_meminj jn jSn)) ev1 ev3 ->
-            exists ev2,
-              inject_sync_event jn ev1 ev2 /\
-              inject_sync_event jSn ev2 ev3 .
-          Proof.
-            intros.
-            destruct ev1.
-            - inv H.
-          Admitted.
-          Lemma inject_mevent_interpolation:
-            forall jn jSn ev1 ev3,
-            (inject_mevent (compose_meminj jn jSn)) ev1 ev3 ->
-            exists ev2,
-              inject_mevent jn ev1 ev2 /\
-              inject_mevent jSn ev2 ev3 .
-          Proof.
-            intros.
-            destruct ev1.
-            - inv H.
-              eapply inject_mem_event_interpolation in H3.
-              normal_hyp; repeat (econstructor; eauto).
-            - inv H.
-              eapply inject_mem_sync_interpolation in H3.
-              normal_hyp; repeat (econstructor; eauto).
-          Qed.
-              
-          
-          Lemma list_inject_mevent_interpolation:
-            forall jn jSn tr1 tr3,
-            Forall2 (inject_mevent (compose_meminj jn jSn)) tr1 tr3 ->
-            exists tr2,
-              Forall2 (inject_mevent jn) tr1 tr2 /\
-              Forall2 (inject_mevent jSn) tr2 tr3 .
-          Proof.
-            intros ?? tr1.
-            induction tr1.
-            - intros tr3 HH; inv HH.
-              econstructor; eauto.
-            - intros tr3 HH; inv HH.
-              eapply IHtr1 in H3.
-              eapply inject_mevent_interpolation in H1.
-              normal_hyp.
-              eexists; repeat (econstructor; eauto).
-          Qed.            
-Lemma inject_mevent_compose:
-              forall j1 j2 t1 t2 t3,
-              inject_mevent j1 t1 t2->
-              inject_mevent j2 t2 t3->
-              inject_mevent (compose_meminj j1 j2) t1 t3.
-            Admitted.
-            Lemma forall_inject_mevent_compose:
-              forall j1 j2 t1 t2 t3,
-              Forall2 (inject_mevent j1) t1 t2->
-              Forall2 (inject_mevent j2) t2 t3->
-              Forall2 (inject_mevent (compose_meminj j1 j2)) t1 t3.
+        forall jn jSn ev1 ev3,
+          (inject_mem_event (compose_meminj jn jSn)) ev1 ev3 ->
+          exists ev2,
+            inject_mem_event jn ev1 ev2 /\
+            inject_mem_event jSn ev2 ev3 .
+      Proof.
+        intros.
+        destruct ev1.
+        - inv H.
+      Admitted.
+      Lemma inject_mem_sync_interpolation:
+        forall jn jSn ev1 ev3,
+          (inject_sync_event (compose_meminj jn jSn)) ev1 ev3 ->
+          exists ev2,
+            inject_sync_event jn ev1 ev2 /\
+            inject_sync_event jSn ev2 ev3 .
+      Proof.
+        intros.
+        destruct ev1.
+        - inv H.
+      Admitted.
+      Lemma inject_mevent_interpolation:
+        forall jn jSn ev1 ev3,
+          (inject_mevent (compose_meminj jn jSn)) ev1 ev3 ->
+          exists ev2,
+            inject_mevent jn ev1 ev2 /\
+            inject_mevent jSn ev2 ev3 .
+      Proof.
+        intros.
+        destruct ev1.
+        - inv H.
+          eapply inject_mem_event_interpolation in H3.
+          normal_hyp; repeat (econstructor; eauto).
+        - inv H.
+          eapply inject_mem_sync_interpolation in H3.
+          normal_hyp; repeat (econstructor; eauto).
+      Qed.
+      
+      
+      Lemma list_inject_mevent_interpolation:
+        forall jn jSn tr1 tr3,
+          Forall2 (inject_mevent (compose_meminj jn jSn)) tr1 tr3 ->
+          exists tr2,
+            Forall2 (inject_mevent jn) tr1 tr2 /\
+            Forall2 (inject_mevent jSn) tr2 tr3 .
+      Proof.
+        intros ?? tr1.
+        induction tr1.
+        - intros tr3 HH; inv HH.
+          econstructor; eauto.
+        - intros tr3 HH; inv HH.
+          eapply IHtr1 in H3.
+          eapply inject_mevent_interpolation in H1.
+          normal_hyp.
+          eexists; repeat (econstructor; eauto).
+      Qed.            
+      Lemma inject_mevent_compose:
+        forall j1 j2 t1 t2 t3,
+          inject_mevent j1 t1 t2->
+          inject_mevent j2 t2 t3->
+          inject_mevent (compose_meminj j1 j2) t1 t3.
+      Admitted.
+      Lemma forall_inject_mevent_compose:
+        forall j1 j2 t1 t2 t3,
+          Forall2 (inject_mevent j1) t1 t2->
+          Forall2 (inject_mevent j2) t2 t3->
+          Forall2 (inject_mevent (compose_meminj j1 j2)) t1 t3.
+      Proof.
+        intros ?? t1.
+        induction t1.
+        - intros. inv H. inv H0. constructor.
+        - intros. inv H. inv H0. constructor; eauto.
+          eapply inject_mevent_compose; eauto.
+      Qed.
+      Lemma match_state_invariant:
+              forall n x3 x4 st1' m1' x1 x2,
+                invariant st1' ->
+                match_state n x3 x4 st1' m1' x1 x2 ->
+                invariant x1.
             Proof.
-              intros ?? t1.
-              induction t1.
-              - intros. inv H. inv H0. constructor.
-              - intros. inv H. inv H0. constructor; eauto.
-                eapply inject_mevent_compose; eauto.
+              induction n.
+              - intros. inv H0; auto.
+              - intros. inv H0. subst_sig.
+                eapply H8.
             Qed.
+            Lemma match_state_cmpt:
+              forall n x3 x4 st1' m1' x1 x2,
+                mem_compatible st1' m1' ->
+                match_state n x3 x4 st1' m1' x1 x2 ->
+                mem_compatible x1 x2.
+            Proof.
+              induction n.
+              - intros. inv H0; auto.
+              - intros. inv H0. subst_sig.
+                eapply H8.
+            Qed.
+            
+      
+      (* Not this lemma can be generalized away from 
+         splicit index and orders (given here by list_lt).
+         Since it's only used once, we live this form for now.
+       *)
+      
       Lemma simulation_inductive_case:
         forall n : nat,
           (forall m : option mem,
-              HybridMachine_simulation_properties
+              simulation_properties_exposed
                 (HybConcSem (Some 0)%nat m)
                 (HybConcSem (Some n) m)
                 invariant
                 mem_compatible
-                (match_state n)) ->
+                (match_state n)
+                list_lt) ->
           (forall m : option mem,
-              HybridMachine_simulation_properties
+              simulation_properties_exposed
                 (HybConcSem (Some n) m)
                 (HybConcSem (Some (S n)) m)
                 invariant
                 mem_compatible
-                (concur_match n)) ->
+                (concur_match n)
+                 (opt_rel' (InjorderX compiler_sim))) ->
           forall m : option mem,
-            HybridMachine_simulation_properties
+            simulation_properties_exposed
               (HybConcSem (Some 0)%nat m)
               (HybConcSem (Some (S n)) m)
               invariant
-                mem_compatible
-                (match_state (S n)).
+              mem_compatible
+              (match_state (S n))
+                list_lt.
       Proof.
         intros n Hsim0 Hsimn m.
-        specialize (Hsim0 m).
-        specialize (Hsimn m).
-        econstructor.
+        specialize (Hsim0 m). destruct Hsim0 as [Hsim0 Hordr0].
+        specialize (Hsimn m). destruct Hsimn as [Hsimn Hordrn].
+        unshelve econstructor;
+          [econstructor| ].
         - !goal (well_founded _).
           eapply list_ord_part_wf.
           eapply Hsimn.
@@ -359,13 +406,14 @@ Lemma inject_mevent_compose:
             admit.
           + normal_hyp; subst.
             assert (Forall2 (inject_mevent (compose_meminj x2 jSn)) tr1 tr2).
-            { admit. (*Need an inject_incr or something about x2. *)
-            }
+            { eapply inject_incr_trace; try eassumption.
+              eapply compose_meminj_inject_incr; eauto. }
             clear H1.
             normal_goal; eauto.
             * econstructor; eauto.
             * right; repeat weak_split auto.
               constructor; auto.
+            * eapply compose_meminj_inject_incr; eauto.
         - intros.
           inv H2; subst_sig.
           eapply list_inject_mevent_interpolation in H3; normal_hyp.
@@ -377,10 +425,12 @@ Lemma inject_mevent_compose:
           + instantiate(1:= x5).
             eapply forall_inject_mevent_compose; eauto.
           + auto.
+          + eapply compose_meminj_inject_incr; eauto.
           + (* add match_state _ st1 m1 st2 m2 -> invariant st2 *)
-            admit.
+            eapply match_state_invariant; eauto.
+                
           + (* add match_state _ st1 m1 st2 m2 -> mem_compat st2 m2 *)
-            admit.
+            eapply match_state_cmpt; eauto.
           + eauto.
           + eauto.
           + eauto.
@@ -397,18 +447,18 @@ Lemma inject_mevent_compose:
 
           Unshelve.
           all: assumption.
-      Admitted.
+      Admitted. (* Just one silly admit. *)
 
       
       Context (Hexterns_have_events: Asm_externals_have_events Asm_g).
       Lemma compile_n_threads:
         forall n m,
-          HybridMachine_simulation.HybridMachine_simulation_properties
+          simulation_properties_exposed
             (HybConcSem (Some 0)%nat m)
             (HybConcSem (Some n) m)
             invariant
             mem_compatible
-            (match_state n).
+            (match_state n) list_lt.
       Proof.
         induction n.
         - (*trivial reflexive induction*)
@@ -419,22 +469,39 @@ Lemma inject_mevent_compose:
 
     End CompileNThreads.
 
-    Section CompileInftyThread.
-      Context {Hasm_externals: Asm_externals_have_events Asm_g}.
+    Section Lift.
+      (* We lift states to a different semantics: 
+         The state content is exactly the same, 
+         but the type is of a hybrid machine of higher order.
+       *)
+
       
+      (* Create a database for eauto and autorewrite
+       *)
+      Create HintDb lift.
+      Tactic Notation "lift":= eauto with lift.
+      Tactic Notation "rw_lift":= autorewrite with lift.
+
+
+      (** *Definitions*)
       Definition lift_state': forall {on on'},
           ThreadPool on -> ThreadPool on'.
-      Proof.
-        intros; inv X; econstructor; eauto.
-      Defined.
-      
+      Proof.  intros; inv X; econstructor; eauto. Defined.
       Inductive lift_state: forall on, ThreadPool on -> forall on', ThreadPool on' -> Prop:=
       | build_lift_state: forall on on' st st',
           st' = lift_state' st -> lift_state on st on' st'.
+      Hint Constructors lift_state: lift.
+
+
+      (** *Core lemmas *)
+      Lemma lift_state_refl:
+        forall n st, @lift_state' n n st = st.
+      Proof. intros; destruct st; simpl. f_equal. Qed.
+      Hint Resolve lift_state_refl: lift.
       Lemma lift_contains:
         forall {on on'} st j,
-          ThreadPool.containsThread st j <->
-          ThreadPool.containsThread (@lift_state' on on' st) j.
+          OrdinalPool.containsThread st j <->
+          OrdinalPool.containsThread (@lift_state' on on' st) j.
       Proof.
         intros. simpl.
         unfold OrdinalPool.containsThread; simpl.
@@ -442,59 +509,557 @@ Lemma inject_mevent_compose:
       Qed.
       Lemma lift_contains1:
         forall {on on'} st j,
-          ThreadPool.containsThread st j ->
-          ThreadPool.containsThread (@lift_state' on on' st) j.
+          OrdinalPool.containsThread st j ->
+          OrdinalPool.containsThread (@lift_state' on on' st) j.
+      Proof. intros; eapply lift_contains in H; eauto. Qed.
+      Hint Resolve lift_contains1: lift.
+      (* this version is better to use in statement of lemmas to rewrite*)
+      Lemma unlift_cnt:
+        forall on on' {st j},
+          OrdinalPool.containsThread (@lift_state' on on' st) j ->
+          OrdinalPool.containsThread st j.
       Proof. intros; eapply lift_contains in H; eauto. Qed.
       Lemma lift_contains2:
         forall {on on'} st j,
-          ThreadPool.containsThread (@lift_state' on on' st) j ->
-          ThreadPool.containsThread st j.
+          OrdinalPool.containsThread (@lift_state' on on' st) j ->
+          OrdinalPool.containsThread st j.
       Proof. intros; eapply lift_contains in H; eauto. Qed.
+      Lemma lift_getC:
+        forall on on' st tid
+          (Htid: OrdinalPool.containsThread st tid)
+          (Htid': OrdinalPool.containsThread (@lift_state' on on' st) tid),
+          OrdinalPool.getThreadC Htid' = OrdinalPool.getThreadC Htid.
+      Proof.
+        intros. destruct st; simpl in *.
+        replace Htid' with Htid by apply Axioms.proof_irr; auto.
+      Qed.
+      Lemma lift_getC':
+        forall on on' st tid
+          (Htid': OrdinalPool.containsThread (@lift_state' on on' st) tid),
+          OrdinalPool.getThreadC Htid' = OrdinalPool.getThreadC (unlift_cnt on on' Htid').
+      Proof. intros; eapply lift_getC; auto. Qed.
+      Hint Rewrite lift_getC': lift.
+      Lemma lift_getR:
+        forall on on' st tid
+          (Htid: OrdinalPool.containsThread st tid)
+          (Htid': OrdinalPool.containsThread (@lift_state' on on' st) tid),
+          OrdinalPool.getThreadR Htid' = OrdinalPool.getThreadR Htid.
+      Proof.
+        intros. destruct st; simpl in *.
+        replace Htid' with Htid by apply Axioms.proof_irr; auto.
+      Qed.
+      Lemma lift_getR':
+        forall on on' st tid
+          (Htid': OrdinalPool.containsThread (@lift_state' on on' st) tid),
+          OrdinalPool.getThreadR Htid' = OrdinalPool.getThreadR (unlift_cnt on on' Htid').
+      Proof. intros; eapply lift_getR; auto. Qed.
+      Hint Rewrite lift_getR': lift.
+      Lemma lift_lockRes:
+        forall on on' st l,
+          OrdinalPool.lockRes (@lift_state' on on' st) l =
+          OrdinalPool.lockRes st l.
+      Proof.
+        intros; destruct st; simpl.
+        unfold OrdinalPool.lockRes; simpl; reflexivity.
+      Qed.
+      Hint Rewrite lift_lockRes: lift.
+      
+      
+      
+      
+      Lemma lift_invariant:
+        forall hb1 hb2 st st',
+          lift_state hb1 st hb2 st' ->
+          invariant st -> invariant st'.
+      Admitted.
+      Lemma lift_invariant':
+        forall hb1 hb2 st,
+          invariant st -> invariant (@lift_state' hb1 hb2 st).
+      Proof.
+        intros. eapply lift_invariant; eauto.
+        econstructor; eauto.
+      Qed.
+      Hint Resolve lift_invariant': lift.
+      Lemma lift_cmpt:
+        forall hb1 hb2 st m,
+          mem_compatible st m ->
+          mem_compatible (@lift_state' hb1 hb2 st) m.
+      Proof.
+        intros. inv H; simpl in *.
+        econstructor; simpl;
+          intros; simpl; autorewrite with lift in *;
+            clean_proofs_goal; eauto.
+      Qed.
+      Hint Resolve lift_cmpt: lift.
+      
+      Lemma lift_state_idempotent:
+        forall base n top st,
+          @lift_state' (Some n) top
+                       (@lift_state' base (Some n) st) =
+          @lift_state' base top st.
+      Proof. intros. destruct st; eauto. Qed.
+      Hint Rewrite lift_state_idempotent: lift.
+
+      
+      (* for some reason, getC doesn't autorewrite
+         it seems like it unifies on = on' before rewriteting,
+         unless given explicitly...
+       *)
+      Ltac rewrite_getC:=
+        match goal with
+          |- @OrdinalPool.getThreadC
+              _ _ ?i
+              (@lift_state' ?on ?on'  ?st) ?cnt
+            = _ =>
+          rewrite (lift_getC' on on');
+          clean_proofs_goal; lift
+        end.
+      
+      Ltac lift_tac:=
+        autorewrite with lift in *;
+        try rewrite_getC; 
+        clean_proofs_goal; lift.
+      
+      
+      Lemma unlift_permMapLt:
+        forall on on' {st tid m}
+          {Htid': ThreadPool.containsThread
+                    (@lift_state' on on' st) tid}
+          (Hlt': permMapLt
+                   (thread_perms (lift_state' st) tid Htid')
+                   (getMaxPerm m)),
+          permMapLt
+            (thread_perms st tid (unlift_cnt _ _ Htid'))
+            (getMaxPerm m).
+      Proof. intros; lift_tac. Qed.
+      Hint Resolve @unlift_permMapLt: lift.
+      Lemma unlift_permMapLt_lock:
+        forall on on' {st tid m}
+               {Htid': ThreadPool.containsThread
+                         (@lift_state' on on' st) tid}
+               (Hlt': permMapLt
+                        (lock_perms (lift_state' st) tid Htid')
+                        (getMaxPerm m)),
+          permMapLt
+            (lock_perms st tid (unlift_cnt _ _ Htid'))
+            (getMaxPerm m).
+      Proof. intros; lift_tac. Qed.
+      Hint Resolve @unlift_permMapLt_lock: lift.
+      
+      Lemma lift_restrPermMap:
+        forall on on' st tid m
+               (Htid': ThreadPool.containsThread
+                         (@lift_state' on on' st) tid)
+               (Hlt': permMapLt
+                        (thread_perms (lift_state' st) tid Htid')
+                        (getMaxPerm m)),
+          restrPermMap Hlt' =
+          restrPermMap (unlift_permMapLt _ _ Hlt').
+      Proof.
+        intros.
+        eapply restre_equiv_eq; lift_tac;
+          reflexivity.
+      Qed.
+      Hint Rewrite lift_restrPermMap: lift.
+      
+      Lemma lift_restrPermMap_lk:
+        forall on on' st tid m
+          (Htid': ThreadPool.containsThread
+                    (@lift_state' on on' st) tid)
+          (Hlt': permMapLt
+                   (lock_perms (lift_state' st) tid Htid')
+                   (getMaxPerm m)),
+          restrPermMap Hlt' =
+          restrPermMap (unlift_permMapLt_lock _ _ Hlt').
+      Proof.
+        intros.
+        eapply restre_equiv_eq; lift_tac;
+          reflexivity.
+      Qed.
+      Hint Rewrite lift_restrPermMap_lk: lift.
+
+      
+      
+      
+      (** *Regular lemmas
+          i.e. don't go in the database 
+       *)
       Lemma lift_unique_Krun:
         forall {on on'} st i,
           HybridMachineSig.unique_Krun st i <->
           HybridMachineSig.unique_Krun (@lift_state' on on' st) i.
       Proof.
-        intros; split; intros ** ? **.
-        - unshelve eapply H; eauto.
-          eapply (@lift_contains on on' st j); auto.
-          simpl. match_case; simpl.
-          clear - H0.
+        intros; split; intros ** ? **; simpl in *.
+        - unshelve eapply H; eauto; simpl.
+          eapply lift_contains2; eauto.
           destruct st; simpl in *.
-          replace (c0 cnti) with cnti by apply Axioms.proof_irr.
-          rewrite H0.
-          reflexivity.
-        - unshelve eapply H; eauto.
-          eapply (@lift_contains on on' st j); auto.
-          simpl. match_case; simpl.
-          clear - H0.
+          rewrite <- H0; f_equal.
+          clean_proofs_goal; reflexivity.
+        - unshelve eapply H; eauto; simpl.
+          lift.
           destruct st; simpl in *.
-          replace (c cnti) with (cnti) by apply Axioms.proof_irr.
-          rewrite H0.
-          reflexivity.
+          rewrite <- H0; f_equal.
+          clean_proofs_goal; reflexivity.
       Qed.
 
-      
-      Lemma lift_invariant:
-        forall hb1 hb2 st st',
-          lift_state hb1 st hb2 st' ->
-          invariant st ->
-          invariant st'.
-      Admitted.
-      Lemma lift_cmpt:
-        forall hb1 hb2 st st' m,
-          lift_state hb1 st hb2 st' ->
-          mem_compatible st m ->
-          mem_compatible st' m.
-      Admitted.
+      Lemma lift_updThread:
+        forall on on' st tid
+          (Htid: ThreadPool.containsThread st tid)
+          (Htid': ThreadPool.containsThread (@lift_state' on on' st) tid)
+          c res st',
+          OrdinalPool.updThread Htid c res = st' ->
+          OrdinalPool.updThread Htid' c res = lift_state' st'.
+      Proof.
+        intros.
+        subst st'. destruct st; simpl.
+        unfold OrdinalPool.updThread; simpl.
+        f_equal.
+      Qed.
+      Lemma lift_updThread':
+        forall on on' st tid
+               (Htid': ThreadPool.containsThread (@lift_state' on on' st) tid)
+               c res st',
+          OrdinalPool.updThread (unlift_cnt on on' Htid') c res = st' ->
+          OrdinalPool.updThread Htid' c res = lift_state' st'.
+      Proof.
+        intros.
+        subst st'. destruct st; simpl.
+        unfold OrdinalPool.updThread; simpl.
+        f_equal.
+      Qed.
+      Hint Resolve lift_updThread: lift.
+      Hint Rewrite lift_updThread' using eauto: lift.
 
+      Lemma lift_updThreadC:
+        forall on on' st tid
+               (Htid: ThreadPool.containsThread st tid)
+               (Htid': ThreadPool.containsThread (@lift_state' on on' st) tid)
+               res st',
+          OrdinalPool.updThreadC Htid res = st' ->
+          OrdinalPool.updThreadC Htid' res = lift_state' st'.
+      Proof.
+        intros.
+        subst st'. destruct st; simpl in *.
+        unfold lift_state' in *.
+        unfold OrdinalPool.updThreadC; simpl.
+        f_equal.
+      Qed.
+      Hint Resolve lift_updThreadC: lift.
+      Hint Rewrite lift_updThreadC: lift.
+      
+      Notation MachineSig_n on:= (@DryHybridMachineSig
+                                    (@HybridSem CC_correct Args on) (TP on)).
+      
+      Lemma lift_install_perm:
+        forall on on' st tid m m'
+          (Htid: ThreadPool.containsThread st tid)
+          (Htid': ThreadPool.containsThread (@lift_state' on on' st) tid)
+          (Hcmpt : HybridMachineSig.mem_compatible st m)
+          (Hcmpt' : HybridMachineSig.mem_compatible (@lift_state' on on' st) m),
+          @HybridMachineSig.install_perm _ _ _
+                                         (MachineSig_n on)  _ _ _ Hcmpt Htid m' ->
+          @HybridMachineSig.install_perm _ _ _
+                                         (MachineSig_n on')  _ _ _ Hcmpt' Htid' m'.
+      Proof.
+        simpl in *. 
+        unfold HybridMachineSig.install_perm, install_perm; simpl;
+          unfold install_perm; intros.
+        clean_proofs_goal.
+        subst m'; f_equal.
+        simpl.
+        eapply synchronisation_lemmas.restrPermMap_access_equiv.
+        unfold thread_perms; simpl.
+        remember (OrdinalPool.getThreadR Htid) as X.
+        symmetry in HeqX.
+        erewrite lift_getR; auto.
+        subst X; reflexivity.
+      Qed.
+      Lemma lift_install_perm':
+        forall on on' (st: OrdinalPool.t) tid m  m'
+          (Htid: OrdinalPool.containsThread st tid)
+          (Htid': OrdinalPool.containsThread (@lift_state' on on' st) tid)
+          (Hcmpt : @mem_compatible _ (@OrdinalPool.OrdinalThreadPool
+                                        _
+                                        (@HybridSem CC_correct Args on)) st m)
+          (Hcmpt' : mem_compatible (@lift_state' on on' st) m),
+          install_perm _ _ _ Hcmpt Htid m' ->
+          install_perm  _ _ _ Hcmpt' Htid' m'.
+      Proof. eapply lift_install_perm. Qed.
+      Hint Resolve lift_install_perm': lift.
+      Hint Resolve lift_install_perm: lift.
+      
+      Definition hb_le (hb1 hb2: option nat):=
+        match hb1, hb2 with
+        | Some n1, Some n2 => (n1 <= n2)%nat
+        | _, None => True
+        | _ , _ => False
+        end.
+      Lemma  lt_op_hb_le:
+        forall tid on1 on2,
+          lt_op tid on1 ->
+          hb_le on1 on2 ->
+          lt_op tid on2.
+      Proof.
+        intros. unfold hb_le in H0.
+        repeat match_case in H0; subst; simpl in *.
+        omega.
+      Qed.
+      
+      Lemma lift_initial_core:
+        forall on on' tid m c m' vf arg,
+          lt_op tid on -> hb_le on on' ->
+          initial_core (sem_coresem (HybridSem on)) tid m c m' vf arg ->
+          initial_core (sem_coresem (HybridSem on')) tid m
+                       c m' vf arg.
+      Proof.
+        unfold HybridSem; simpl.
+        intros. simpl in H1.
+        unfold initial_core_sum in H1.
+        match_case in H1.
+        - normal. contradict H1; apply H.
+        - simpl. normal; eauto.
+          eapply lt_op_hb_le; eauto.
+      Qed.
+      Hint Resolve lift_initial_core: lift.
+      
+      Definition ThreadPool_num_threads {hb1} (st:ThreadPool hb1): nat.
+        apply pos.n.
+        eapply @OrdinalPool.num_threads.
+        simpl in st. eauto.
+      Defined.
+      
+      Lemma  lt_op_lt:
+        forall tid x on2,
+          lt_op x on2 ->
+          (tid < x)%nat ->
+          lt_op tid on2.
+      Proof.
+        intros. unfold lt_op in *.
+        match_case; eauto.
+        omega.
+      Qed.
+      Lemma cnt_pos_threads_lt:
+        forall hb (st: ThreadPool (hb)) tid, 
+          ThreadPool.containsThread st tid ->
+          (tid < ThreadPool_num_threads st)%nat.
+      Proof.
+        unfold ThreadPool_num_threads in *.
+        intros. 
+        apply (Nat.lt_le_trans _ (S tid)); try omega.
+        exploit (@ssrnat.leP (S tid) (pos.n (OrdinalPool.num_threads st))). 
+        hnf in H. intros HH; inv HH; auto.
+        rewrite H in H0; congruence.
+      Qed.
+      Lemma lift_start_thread:
+        forall on on' m st st' m' tid
+          (Htid: ThreadPool.containsThread st tid)
+          (Htid': ThreadPool.containsThread (lift_state' st) tid)
+          (Hltop: lt_op (ThreadPool_num_threads st) on)
+          (Hhb_le: hb_le on on'),
+          start_thread(machineSig:=MachineSig_n on)
+                      m Htid st' m' ->
+          start_thread(machineSig:=MachineSig_n on')
+                      m Htid' (lift_state' st') m'.
+      Proof.
+        intros.
+        inv H; econstructor; simpl in *;
+          lift_tac.
+        - instantiate (1:= c_new).
+          hnf in Hinitial.
+          match_case in Hinitial.
+          normal_hyp.
+          contradict H.
+          + eapply lt_op_lt; eauto.
+            eapply cnt_pos_threads_lt; auto.
+          + simpl. normal; eauto.
+            eapply lt_op_hb_le; eassumption.
+        - unfold add_block; simpl.
+          autorewrite with lift; simpl.
+          erewrite lift_updThread; eauto; simpl.
+          autorewrite with lift in *;
+            clean_proofs_goal; lift.
+
+          Unshelve.
+          simpl; lift.
+      Qed.
+      Lemma lift_resume_thread:
+        forall on on' m st st' tid
+          (Htid: ThreadPool.containsThread st tid)
+          (Htid': ThreadPool.containsThread (lift_state' st) tid)
+          (Hltop: lt_op (ThreadPool_num_threads st) on)
+          (Hhb_le: hb_le on on'),
+          resume_thread(machineSig:=MachineSig_n on)
+                       m Htid st' ->
+          resume_thread(machineSig:=MachineSig_n on')
+                       m Htid' (lift_state' st').
+      Proof.
+        intros.
+        inv H; econstructor; simpl in *; lift_tac.
+        erewrite lift_updThreadC; eauto; reflexivity.
+
+        Unshelve.
+        all: simpl; lift.
+        
+      Qed.
+      
+      Lemma lift_suspend_thread:
+        forall on on' m st st' tid
+          (Htid: ThreadPool.containsThread st tid)
+          (Htid': ThreadPool.containsThread (lift_state' st) tid)
+          (Hltop: lt_op (ThreadPool_num_threads st) on)
+          (Hhb_le: hb_le on on'),
+          suspend_thread(machineSig:=MachineSig_n on)
+                        m Htid st' ->
+          suspend_thread(machineSig:=MachineSig_n on')
+                        m Htid' (lift_state' st').
+      Proof.
+        intros.
+        inv H; econstructor; simpl in *;lift_tac.
+        erewrite lift_updThreadC; eauto; reflexivity.
+
+        Unshelve.
+        all: simpl; lift.
+      Qed.
+      Lemma lift_syncStep:
+        forall on on' m st m' st' tid ev
+          (Htid: ThreadPool.containsThread st tid)
+          (Htid': ThreadPool.containsThread (@lift_state' on on' st) tid)
+          (Hltop: lt_op (ThreadPool_num_threads st) on)
+          (Hcmpt : @mem_compatible _ (@OrdinalPool.OrdinalThreadPool
+                                        _
+                                        (@HybridSem CC_correct Args on)) st m)
+          (Hcmpt' : mem_compatible (lift_state' st) m),
+          syncStep true Htid Hcmpt st' m' ev ->
+          syncStep true Htid' Hcmpt' (lift_state' st') m' ev.
+      Proof.
+        intros.
+        inv H;
+          [ econstructor 1 |
+            econstructor 2 |
+            econstructor 3 |
+            econstructor 4 |
+            econstructor 5 |
+            econstructor 6]; eauto;
+            simpl in *; lift_tac; (* 7! goals *)
+              try solve[destruct st; simpl; eauto];
+              clean_proofs; eauto.
+        1,2: rewrite <- Hstore; f_equal;
+          eapply restre_equiv_eq; lift_tac;
+            reflexivity.
+
+        Unshelve.
+        all: simpl in *; lift_tac. 
+      Qed.
+      Lemma lift_thread_step:
+        forall on on' tge U st st' m2 x1 m,
+          machine_semantics.thread_step
+            (HybConcSem on m) tge U st m2 st' x1 ->
+          machine_semantics.thread_step
+            (HybConcSem on' m) tge U (@lift_state' on on' st) m2
+            (@lift_state' on on' st') x1.
+      Proof.
+        intros.
+        unshelve (inv H; econstructor; eauto);
+                  try eapply lift_contains1; eauto;
+                    simpl in *; lift.
+        inv Htstep; simpl in *;
+          econstructor; simpl in *; lift_tac.
+        clean_proofs_goal. lift.
+        simpl.
+        unfold OrdinalPool.updThread; simpl in *.
+        rw_lift. destruct st; f_equal.
+      Qed.
+      Lemma lift_thread_Nstep:
+        forall on on' tge x
+          (U : list nat) (st st' : ThreadPool on) (m2 x1 : mem) (m : option mem),
+          machine_semantics_lemmas.thread_stepN (HybConcSem on m) tge x U st m2 st' x1 ->
+          machine_semantics_lemmas.thread_stepN (HybConcSem on' m) tge x U 
+                                                (lift_state' st) m2 (lift_state' st') x1.
+        intros until x. induction x.
+        
+        - intros. inv H; simpl. reflexivity.
+        - intros.
+          simpl in H; normal_hyp.
+          do 2 eexists; split; eauto.
+          simpl; eauto.
+          eapply lift_thread_step; eauto.
+
+          Unshelve.
+          all: auto.
+      Qed.
+      Lemma lift_thread_step_star:
+        forall on on' tge U st st' m2 x1 m,
+          machine_semantics_lemmas.thread_step_star
+            (HybConcSem on m) tge U st m2 st' x1 ->
+          machine_semantics_lemmas.thread_step_star
+            (HybConcSem on' m) tge U (@lift_state' on on' st) m2
+            (@lift_state' on on' st') x1.
+      Proof.
+        intros. inv H. exists x.
+        apply lift_thread_Nstep; auto.
+      Qed.
+      
+      Lemma lift_thread_step_plus:
+        forall on on' tge U st st' m2 x1 m,
+          machine_semantics_lemmas.thread_step_plus
+            (HybConcSem on m) tge U st m2 st' x1 ->
+          machine_semantics_lemmas.thread_step_plus
+            (HybConcSem on' m) tge U (@lift_state' on on' st) m2
+            (@lift_state' on on' st') x1.
+      Proof.
+        intros. inv H. exists x.
+        eapply lift_thread_Nstep; auto.
+      Qed.
+        
+      Lemma lift_machine_step:
+        forall on on' tge U tr2 st st' m2 U' x x1 m
+          (Hhb_le: hb_le on on')
+          (Hltop: lt_op (ThreadPool_num_threads st) on),
+          machine_semantics.machine_step
+            (HybConcSem on m) tge U tr2 st m2 U' x st' x1 ->
+          machine_semantics.machine_step
+            (HybConcSem on' m) tge U tr2 (@lift_state' on on' st) m2 U' x
+            (@lift_state' on on' st') x1.
+      Proof.
+        intros. unshelve (inv H;
+                          [ econstructor 1 |
+                            econstructor 2 |
+                            econstructor 3 |
+                            econstructor 4 |
+                            econstructor 5]; eauto);
+                  try eapply lift_contains1; eauto;
+                    simpl in *; lift.
+        - eapply lift_start_thread; eauto.
+        - eapply lift_resume_thread; eauto.
+        - eapply lift_suspend_thread; eauto.
+        - eapply lift_syncStep; eauto.
+          
+        - destruct Htid; [left|right].
+          + intros HH; apply H; eapply unlift_cnt; eauto.
+          + normal; lift_tac.
+            
+            Unshelve.
+            all: lift.
+      Qed.
+      
+    End Lift.
+    
+    Section CompileInftyThread.
+      Context {Hasm_externals: Asm_externals_have_events Asm_g}.
+
+      
+      Definition self_simulates:
+        forall n, ThreadPool (Some n) -> mem -> Prop:=
+        fun _ _ _ => True.
       
       Inductive infty_match:
         nth_index -> meminj ->
         ThreadPool (Some 0)%nat -> mem ->
         ThreadPool None -> mem -> Prop:=
       | Build_infty_match:
-          forall n cd j st0 m0 stn mn st,
+          forall n cd j st0 m0 stn mn st
+            (Hself_inj:  self_simulates n stn mn)
+            (Hhb_bound: (0 < ThreadPool_num_threads st0 < n)%nat),
             match_state n cd j st0 m0 stn mn ->
             lift_state (Some n) stn None st ->
             infty_match cd j st0 m0 st mn.
@@ -516,7 +1081,197 @@ Lemma inject_mevent_compose:
       (* Follows from any initial diagram and a missing lemma showing that the initial state
         can be "lifted" (lift_state) *)
       Admitted.
+      
+      Lemma self_simulates_match:
+        forall hb1 (st:ThreadPool (Some hb1)) m,
+          (ThreadPool_num_threads st < hb1)%nat ->  
+          self_simulates hb1 st m ->
+          concur_match hb1 None (Mem.flat_inj (Mem.nextblock m)) st m (lift_state' st) m.
+      Proof.
+      Admitted.
+      Lemma lift_self_simulates:
+        forall hb1 hb2 st m, 
+          self_simulates hb1 st m ->
+          (ThreadPool_num_threads st < hb1)%nat -> 
+          (hb1 <= hb2)%nat ->
+          self_simulates hb2 (lift_state' st) m.
+      Admitted.
+      Lemma machine_step_preserves_self_simulates:
+        forall n m0 ge U tr st m U' tr' st' m',
+          self_simulates n st m ->
+          machine_semantics.machine_step (HybConcSem (Some n) m0)
+                                         ge U tr st m U' tr' st' m' ->
+          self_simulates n st' m'.
+      Proof.
+      Admitted.
+      Fixpoint Nones {A} (n:nat):=
+        match n with
+          O => nil
+        | S n' => @None A :: (Nones n')
+        end.
+      
+      Definition mappedblocks f m2:=
+        forall (b b' : block) (delta : Z),
+          f b = Some (b', delta) -> Mem.valid_block m2 b'.
+      Lemma mappedblocks_compose_meminj:
+        forall f m2,
+          mappedblocks f m2 ->
+          f = (compose_meminj f (Mem.flat_inj (Mem.nextblock m2))).
+      Proof.
+        intros.
+        unfold compose_meminj.
+        unfold Mem.flat_inj,compose_meminj.
+        intros.
+        extensionality b; simpl.
+        repeat match_case. subst.
+        - match_case in Heqo0; subst.
+          inv Heqo0. repeat f_equal; omega.
+        - match_case in Heqo0; subst.
+          apply H in Heqo.
+          clear Heqs.
+          contradict n. apply Heqo.
+      Qed.
+      Lemma match_state_num_threads:
+        forall n ocd mu st1 m1 st2 m2,
+          match_state n ocd mu st1 m1 st2 m2 ->
+          ThreadPool_num_threads st1 =
+          ThreadPool_num_threads st2.
+      Proof.
+        induction n.
+        - intros. inv H. subst_sig; reflexivity.
+        - intros * H. inv H. subst_sig.
+          etransitivity.
+          eapply IHn; eauto.
+          unfold ThreadPool_num_threads.
+          apply same_length in H7.
+          f_equal.
+          destruct tpn, st2; simpl in *; auto.
+      Qed.
+      Lemma mappedblocks_flat:
+        forall m2, 
+          mappedblocks (Mem.flat_inj (Mem.nextblock m2)) m2.
+      Proof.
+        intros ** ? ** . 
+        unfold Mem.flat_inj in *.
+        match_case in H.
+      Qed.
+      Lemma concur_match_mappedblocks:
+        forall n ocd mu st1 m1 st2 m2,
+          (0 < ThreadPool_num_threads st1)%nat -> 
+          concur_match n ocd mu st1 m1 st2 m2 ->
+          mappedblocks mu m2.
+      Proof.
+        intros.
+        assert (Hcnt1:ThreadPool.containsThread st1 0).
+        { unfold ThreadPool.containsThread; simpl.
+          unfold OrdinalPool.containsThread.
+          unfold ThreadPool_num_threads in *.
+          destruct st1; subst; simpl.
+          clear - H.
+          pose proof (@ssrnat.leP 1 (pos.n num_threads)).
+          inv H0; auto. }
+        assert (Hcnt2:ThreadPool.containsThread st2 0).
+        { eapply contains12; eauto. }
 
+        assert (Hlt1:permMapLt (fst (ThreadPool.getThreadR Hcnt1)) (getMaxPerm m1)).
+        { eapply memcompat1 in H0. apply H0. }
+        assert (Hlt2:permMapLt (fst (ThreadPool.getThreadR Hcnt2)) (getMaxPerm m2)).
+        { eapply memcompat2 in H0. apply H0. }
+
+        unshelve eapply INJ_threads in H0; try eapply Hcnt1; eauto.
+        intros ? **.
+        eapply Mem.mi_mappedblocks in H0; eauto.
+      Qed.
+      Lemma match_state_mappedblocks:
+        forall n ocd mu st1 m1 st2 m2,
+          (0 < ThreadPool_num_threads st1)%nat ->
+          match_state n ocd mu st1 m1 st2 m2 ->
+          mappedblocks mu m2.
+      Proof.
+        intros. inv H0; subst_sig.
+        - 
+          eapply mappedblocks_flat.
+        - intros ? **.
+          unfold compose_meminj in H0.
+          repeat match_case in H0. inv H0.
+          eapply concur_match_mappedblocks; try eapply H10; eauto.
+          erewrite <- match_state_num_threads; eauto.
+      Qed.
+      
+      Lemma pump_match_state:
+        forall m n ocd mu st1 m1 st2 m2
+          (Hpos: (0 < ThreadPool_num_threads st1)%nat),
+          match_state n ocd mu st1 m1 st2 m2 ->
+          self_simulates _ st2 m2 ->
+          (ThreadPool_num_threads st2 < n)%nat -> 
+          (n <= m)%nat ->
+          match_state m ((Nones (m-n)) ++ ocd) mu st1 m1 (lift_state' st2) m2.
+      Proof.
+        intros. 
+        assert (exists x, m = x + n)%nat.
+        { exists (m - n)%nat. omega. }
+        normal_hyp; subst.
+        clear H2.
+        replace (x + n - n)%nat with x by omega.
+        revert n mu ocd st1 st2 m1 m2 Hpos H H1 H0.
+        induction x.
+        - simpl.
+          intros; rewrite lift_state_refl; auto.
+        - intros.
+          exploit IHx; eauto. clear IHx.
+          intros HH.
+          simpl.
+          replace mu with (compose_meminj mu (Mem.flat_inj (Mem.nextblock m2))).
+          2: { symmetry; apply mappedblocks_compose_meminj.
+               eapply match_state_mappedblocks; eauto. }
+
+          simpl.
+          eapply step_match_state; eauto.
+          erewrite <- (lift_state_idempotent (Some n) (x + n) (Some (S (x + n)))).
+          + eapply self_simulates_match; eauto.
+            destruct st2; unfold ThreadPool_num_threads in *; simpl in *.
+            omega.
+      Qed.
+
+            Lemma thread_step_preserves_self_simulates:
+              forall n m0 ge U st m st' m',
+                self_simulates n st m ->
+                machine_semantics.thread_step (HybConcSem (Some n) m0)
+                                               ge U st m st' m' ->
+                self_simulates n st' m'.
+            Proof.
+            Admitted.
+            Lemma thread_step_star_preserves_self_simulates:
+              forall n m0 ge U st m st' m',
+                self_simulates n st m ->
+                machine_semantics_lemmas.thread_step_star (HybConcSem (Some n) m0)
+                                               ge U st m st' m' ->
+                self_simulates n st' m'.
+            Proof.
+              intros. inv H0.
+              revert dependent m.
+              revert U st st' m'.
+              induction x.
+              - simpl. intros. inv H1; assumption.
+              - simpl; intros. normal_hyp.
+                eapply IHx; try eapply H1.
+                eapply thread_step_preserves_self_simulates; eauto.
+                simpl; eassumption.
+
+                Unshelve.
+                all: eauto.
+            Qed.
+            
+            Lemma thread_step_plus_preserves_self_simulates:
+              forall n m0 ge U st m st' m',
+                self_simulates n st m ->
+                machine_semantics_lemmas.thread_step_plus (HybConcSem (Some n) m0)
+                                               ge U st m st' m' ->
+                self_simulates n st' m'.
+            Proof.
+              intros. eapply thread_step_star_preserves_self_simulates; eauto.
+              apply machine_semantics_lemmas.thread_step_plus_star; eassumption.
+            Qed.
       Lemma infinite_step_diagram:
         forall (m : option mem) (sge tge : HybridMachineSig.G)
           (U : list nat) tr1 (st1 : ThreadPool (Some 0)%nat) 
@@ -537,7 +1292,7 @@ Lemma inject_mevent_compose:
                  (HybConcSem None m) tge U st2 m2 st2' m2' \/
                machine_semantics_lemmas.thread_step_star 
                  (HybConcSem None m) tge U st2 m2 st2' m2' /\ 
-               list_lt cd' cd).
+               list_lt cd' cd) /\ inject_incr mu mu' .
       Proof.
       (*Proof sketch:
             infty_match defines an intermediate machine Mn at level n, matching the 0 machine.
@@ -547,7 +1302,69 @@ Lemma inject_mevent_compose:
             [match_states]. Since we increased the hybrid bound (n -> S n) then the new thread 
             is in Asm and [match_states] can be lifted to [infty_match].
        *)
-      Admitted.
+        intros. inv H0.
+        assert (Hsame_num: ThreadPool_num_threads st1' = ThreadPool_num_threads st1).
+        { unfold ThreadPool_num_threads; inv H; simpl; eauto.
+          inv Htstep; simpl; eauto. }
+        
+        pose proof (compile_n_threads Hasm_externals n m) as HH.
+        destruct HH as [HH HHorder]; destruct HH; simpl in HHorder.
+        clear thread_running thread_halted machine_diagram initial_setup.
+        eapply thread_diagram in H; eauto.
+        normal_hyp.
+        normal; eauto.
+        - econstructor; swap 1 3.
+          + eassumption.
+          + rewrite Hsame_num; split; eauto.
+          + destruct H4 as [ ?| [? ?] ];
+              [ eapply thread_step_plus_preserves_self_simulates |
+                eapply thread_step_star_preserves_self_simulates]; eauto.
+          + econstructor; eauto.
+        - inv H3; repeat subst_sig.
+          destruct H4 as [ H4| [H4 ?] ];
+            [ left;eapply lift_thread_step_plus |
+              right; split; try eapply lift_thread_step_star]; eauto.
+      Qed.
+
+      Lemma cnt_pos_threads:
+        forall hb (st: ThreadPool (hb)) tid, 
+          ThreadPool.containsThread st tid ->
+          (0 < ThreadPool_num_threads st)%nat.
+      Proof.
+        unfold ThreadPool_num_threads in *.
+        intros. 
+        apply (Nat.lt_le_trans _ (S tid)); try omega.
+        exploit (@ssrnat.leP (S tid) (pos.n (OrdinalPool.num_threads st))). 
+        hnf in H. intros HH; inv HH; auto.
+        rewrite H in H0; congruence.
+      Qed.
+      
+      Lemma lift_ThreadPool_num_threads:
+        forall  hb cd mu st1 m1 st2 m2,
+          match_state hb cd mu st1 m1 st2 m2 ->
+          ThreadPool_num_threads st2 = ThreadPool_num_threads st1.
+      Proof.
+        unfold ThreadPool_num_threads.
+        induction hb.
+        - simpl; intros; auto. inv H; subst_sig; auto.
+        - intros. inv H; subst_sig.
+          etransitivity; swap 1 2.
+          eapply IHhb; eauto.
+          apply same_length in H7; rewrite H7; reflexivity.
+      Qed.
+      
+      
+      Lemma machine_step_has_threads:
+        forall n m0 ge U tr st m U' tr' st' m',
+          (0 < ThreadPool_num_threads st)%nat ->
+          machine_semantics.machine_step (HybConcSem (Some n) m0)
+                                         ge U tr st m U' tr' st' m' ->
+          (0 < ThreadPool_num_threads st')%nat.
+      Proof.
+        intros. unfold ThreadPool_num_threads in *.
+        inv H0; eauto;
+          inv Htstep; simpl; auto.
+      Qed.  
       Lemma infinite_machine_step_diagram:
         forall (m : option mem) (sge tge : HybridMachineSig.G)
           (U : list nat) (tr1 : HybridMachineSig.event_trace)
@@ -569,125 +1386,59 @@ Lemma inject_mevent_compose:
               infty_match cd' mu' st1' m1' st2' m2' /\
               List.Forall2 (inject_mevent mu') tr1' tr2' /\
               machine_semantics.machine_step (HybConcSem None m) tge U tr2 st2
-                                             m2 U' tr2' st2' m2'.
+                                             m2 U' tr2' st2' m2' /\
+              inject_incr mu mu'.
       Proof.
         intros. inv H0.
-        pose proof (compile_n_threads Hasm_externals n m) as HH.
+        (* We will move the bound up "pump" 
+           to ensure that it's higher than the number
+           of threads AFTER the step
+         *)
+        set (new_hb:= max n (S (ThreadPool_num_threads st1'))).
+        assert (Hnew_hb_spec1: (n <= new_hb)%nat) by apply Nat.le_max_l.
+        
+        rename stn into old_stn.
+        exploit (pump_match_state new_hb); eauto.
+        { apply Hhb_bound. }
+        { erewrite lift_ThreadPool_num_threads; eauto.
+          apply Hhb_bound. }
+        remember (lift_state' old_stn) as stn.
+
+        rename H3 into H3'.
+        assert (H3: lift_state _ stn None st2).
+        { econstructor; subst.
+          erewrite lift_state_idempotent.
+          inv H3'; repeat subst_sig; auto. }
+        clear H3'.
+
+        eapply (lift_self_simulates n new_hb) in Hself_inj; eauto.
+        2:{ erewrite lift_ThreadPool_num_threads; eauto. apply Hhb_bound. }
+        rewrite <- Heqstn in Hself_inj.
+        clear H2 Heqstn old_stn; intros H2.
+
+        (* Now everything is the same, but with a larger bound!*)
+        
+        pose proof (compile_n_threads Hasm_externals new_hb m) as HH.
+        destruct HH as [HH _].
         eapply machine_diagram in HH; eauto.
         normal_hyp.
         normal; eauto.
-        - econstructor; eauto. econstructor; eauto.
-        - Lemma lift_machine_step:
-            forall on on' tge U tr2 st st' m2 U' x x1 m,
-              machine_semantics.machine_step
-              (HybConcSem on m) tge U tr2 st m2 U' x st' x1 ->
-            machine_semantics.machine_step
-              (HybConcSem on' m) tge U tr2 (@lift_state' on on' st) m2 U' x
-              (@lift_state' on on' st') x1.
-          Proof.
-            intros. unshelve (inv H;
-                      [ econstructor 1 |
-                        econstructor 2 |
-                        econstructor 3 |
-                        econstructor 4 |
-                        econstructor 5]; eauto);
-                      try eapply lift_contains1; eauto;
-                        simpl in *.
-            - eapply lift_cmpt; eauto.
-              econstructor; auto.
-            -
-              Notation MachineSig_n on:= (@DryHybridMachineSig
-                                  (@HybridSem CC_correct Args on) (TP on)).
-              Lemma lift_getC:
-                forall on on' st tid X
-                  (Htid: ThreadPool.containsThread st tid)
-                  (Htid': ThreadPool.containsThread (@lift_state' on on' st) tid),
-                  ThreadPool.getThreadC Htid = X ->
-                  ThreadPool.getThreadC Htid' = X.
-              Proof.
-                intros. destruct st; simpl in *.
-                replace Htid' with Htid by apply Axioms.proof_irr; auto.
-              Qed.
-              Lemma lift_getR:
-                forall on on' st tid X
-                  (Htid: ThreadPool.containsThread st tid)
-                  (Htid': ThreadPool.containsThread (@lift_state' on on' st) tid),
-                  ThreadPool.getThreadR Htid = X ->
-                  ThreadPool.getThreadR Htid' = X.
-              Proof.
-                intros. destruct st; simpl in *.
-                replace Htid' with Htid by apply Axioms.proof_irr; auto.
-              Qed.
-              Lemma lift_getR':
-                forall on on' st tid
-                  (Htid: ThreadPool.containsThread st tid)
-                  (Htid': ThreadPool.containsThread (@lift_state' on on' st) tid),
-                  ThreadPool.getThreadR Htid' = 
-                  ThreadPool.getThreadR Htid.
-              Proof.
-                intros. destruct st; simpl in *.
-                replace Htid' with Htid by apply Axioms.proof_irr; auto.
-              Qed.
-              Lemma lift_start_thread:
-                forall on on' m st m' tid
-                (Htid: ThreadPool.containsThread st tid)
-                (Htid': ThreadPool.containsThread (lift_state' st) tid),
-                  start_thread(machineSig:=MachineSig_n on)
-                              m Htid st m' ->
-                start_thread(machineSig:=MachineSig_n on')
-                            m Htid' (lift_state' st) m'.
-              Proof.
-                intros.
-                inv H; econstructor; eauto.
-                eapply lift_getC; eauto.
-                Lemma lift_install_perm:
-                  forall on on' st tid m m'
-                (Htid: ThreadPool.containsThread st tid)
-                (Htid': ThreadPool.containsThread (@lift_state' on on' st) tid)
-                (Hcmpt : HybridMachineSig.mem_compatible st m)
-                (Hcmpt' : HybridMachineSig.mem_compatible (@lift_state' on on' st) m),
-                    @HybridMachineSig.install_perm _ _ _
-                                                   (MachineSig_n on)  _ _ _ Hcmpt Htid m' ->
-                    @HybridMachineSig.install_perm _ _ _
-                                                   (MachineSig_n on')  _ _ _ Hcmpt' Htid' m'.
-                Proof.
-                  unfold HybridMachineSig.install_perm, install_perm; simpl;
-                    unfold install_perm; intros.
-                  clean_proofs.
-                  subst m'; f_equal.
-                  simpl.
-                  eapply synchronisation_lemmas.restrPermMap_access_equiv.
-                  unfold thread_perms; simpl.
-                  remember (OrdinalPool.getThreadR Htid) as X.
-                  symmetry in HeqX.
-                  unshelve eapply lift_getR in HeqX; auto.
-                  subst X; reflexivity.
-                Qed.
-                eapply lift_install_perm; eauto.
-                Lemma lift_initial_core:
-                  forall on on' tid m c m' vf arg,
-                  initial_core (sem_coresem (HybridSem on)) tid m c m' vf arg ->
-                  initial_core (sem_coresem (HybridSem on')) tid m
-                               c m' vf arg.
-                Proof.
-                  unfold HybridSem; simpl.
-                  intros. 
-                  unfold initial_core in H.
-                  unfold sem_coresem in *.
-                  unfold initial_core.
-                  
-              
-              eapply Hcmpt.
-            
-                      try eapply lift_invariant; 
-                      try eapply lift_cmpt; eauto.
-            eapply lift_cmpt.
-            Lemma lift_start_thread:
-              start_thread m2 Htid st' m' ->
-              start_thread m2 ?Htid (lift_state' st') m'.
-            
-        (* Same as the other step diagram.*)
-      Admitted.
+        - econstructor; swap 1 3.
+          + eassumption.
+          + split. 2: apply Nat.le_max_r.
+            eapply machine_step_has_threads; eassumption.
+          + eapply machine_step_preserves_self_simulates; eauto.
+          + econstructor; eauto.
+        - inv H3; repeat subst_sig.
+          instantiate(1:=tge) in H5.
+          unshelve eapply lift_machine_step; try exact None;
+            try assumption.
+          simpl.
+          !goal ((ThreadPool_num_threads stn < new_hb)%nat).
+          { erewrite lift_ThreadPool_num_threads; eauto.
+            omega. }
+      Qed.
+      
 
       Lemma infinite_halted:
         forall (m : option mem) (cd : nth_index) (mu : meminj)
@@ -722,7 +1473,7 @@ Lemma inject_mevent_compose:
         instantiate(1:= machine_semantics.running_thread
                           (HybConcSem (Some n%nat) m)
                           stn i).
-        - clear H st. revert n mu cd i m c1 m1 stn m2 H0.
+        - clear H st Hself_inj Hhb_bound. revert n mu cd i m c1 m1 stn m2 H0.
           induction n.
           + intros. inv H0. subst_sig; reflexivity.
           + intros. inv H0. etransitivity.
@@ -734,17 +1485,19 @@ Lemma inject_mevent_compose:
       Qed.
       Lemma compile_all_threads':
         forall m,
-          HybridMachine_simulation.HybridMachine_simulation_properties
+          simulation_properties_exposed
             (HybConcSem (Some 0)%nat m)
             (HybConcSem None m)
             invariant
             mem_compatible
-            infty_match.
+            infty_match list_lt.
       Proof.
         intros. 
         (*All the proofs use the following lemma*)
         pose proof compile_n_threads as HH.
-        econstructor.
+        
+        unshelve econstructor;
+          [econstructor| ].
         - eapply list_lt_wf.
         - apply initial_infty.
         - apply infinite_step_diagram.
@@ -752,6 +1505,7 @@ Lemma inject_mevent_compose:
             eauto.
         - apply infinite_halted.
         - apply infinite_running.
+        - reflexivity.
       Qed.
       
       Lemma infty_match_invariant:
@@ -759,15 +1513,10 @@ Lemma inject_mevent_compose:
           infty_match cd mu st1 m1 st2 m2 ->
           invariant st1 ->
           invariant st2.
-      Proof.
+      Proof with eauto.
         intros. inv H.
-        assert (invariant stn).
-        { clear H2; revert n st1 m1 st2 m2 cd mu stn H1 H0. clear.
-          induction n; intros.
-          - inv H1; auto.
-          - inv H1; eauto. subst_sig.
-            eapply H8.
-        }
+        assert (invariant stn) by
+        (eapply match_state_invariant; eauto). 
         eapply lift_invariant; eauto.
       Qed.
       Lemma infty_match_cmpt:
@@ -777,14 +1526,10 @@ Lemma inject_mevent_compose:
           mem_compatible st2 m2.
       Proof.
         intros. inv H.
-        assert (mem_compatible stn m2).
-        { revert n  st1 m1 H0  st2 m2 cd mu stn H2 H1. clear.
-          induction n; intros.
-          - inv H1; auto.
-          - inv H1; eauto. subst_sig.
-            eapply H9.
-        }
-        eapply lift_cmpt; eauto.
+        assert (mem_compatible stn m2) by
+            (eapply match_state_cmpt; eauto).
+        inv H2; repeat subst_sig.
+        eapply lift_cmpt; assumption.
       Qed.
       Lemma compile_all_threads:
         forall m,
@@ -800,7 +1545,7 @@ Lemma inject_mevent_compose:
         { eapply compile_all_threads'. }
         - intros; eapply infty_match_invariant; eauto.
         - intros; eapply infty_match_cmpt; eauto.
-      Qed.
+      Qed. 
 
     End CompileInftyThread.
     
