concurrency/compiler/single_thread_simulation_proof.v
@@ -533,7 +533,8 @@ Qed.
                  (HybConcSem (Some (S hb)) m) tge U st2 m2 st2' m2' \/
                machine_semantics_lemmas.thread_step_star
                  (HybConcSem (Some (S hb)) m) tge U st2 m2 st2' m2' /\
-               opt_rel' (InjorderX compiler_sim) cd' cd).
+               opt_rel' (InjorderX compiler_sim) cd' cd) /\
+      inject_incr mu mu'.
       Proof.
         intros.
         inversion H; subst.
@@ -561,8 +562,8 @@ Qed.
           exists (updThread Htid' (Krun (TState Clight.state Asm.state c2'))
                        (getCurPerm m2', snd (getThreadR Htid'))).
           (* new memory is given by the self_simulation. *)
-          exists m2', cd, f'. split; [|split; [|left]].
-          
+          exists m2', cd, f'.
+          repeat weak_split.
           + (*Reestablish the concur_match *)
             simpl.
             move H0 at bottom.
@@ -590,7 +591,7 @@ Qed.
             
           + (* Reestablish inject_mevent *)
             eapply inject_incr_trace; eauto.
-          + (* Construct the step *)
+          + left. (* Construct the step *)
             exists 0%nat; simpl.
             do 2 eexists; split; [|reflexivity].
             dilute_mem m2'.
@@ -600,6 +601,7 @@ Qed.
               eapply H0.
             * simpl; erewrite restr_proof_irr; econstructor; eauto.
             * simpl; repeat (f_equal; try eapply Axioms.proof_irr).
+          + assumption.
           + erewrite restr_proof_irr; eassumption.
             
             
@@ -668,7 +670,7 @@ Qed.
           destruct step as [plus_step | (? & ? & ?)].
           + exists (updThread Htid' (Krun (TState Clight.state Asm.state s2'))
                          (getCurPerm m2', snd (getThreadR Htid'))), m2', (Some i), mu.
-            split; [|split].
+            repeat weak_split.
             * assert (CMatch := H0). inversion H0; subst.
               simpl. admit. (*reestablish concur*)
             * eapply inject_incr_trace; try eassumption.
@@ -683,9 +685,10 @@ Qed.
                  instantiate(1:=Hlt2).
                  eapply step2corestep_plus; simpl in *. 
                  eauto.
+            * apply inject_incr_refl.
                  
           + exists st2, m2, (Some cd'), mu.
-            split; [|split].
+            repeat weak_split.
             * assert (CMatch := H0). inversion H0; subst.
               admit. (*reestablish concur*)
             * eapply inject_incr_trace; try eassumption.
@@ -695,7 +698,7 @@ Qed.
                 exists 0%nat; simpl; auto. }
               { (*order of the index*)
                 constructor; auto.  }
-              
+            * apply inject_incr_refl.
         - (* tid > hb *)
           pose proof (mtch_source _ _ _ _ _ _ H0 _ l Htid (contains12 H0 Htid)) as HH.
           simpl in *.
@@ -719,7 +722,7 @@ Qed.
           exists (updThread Htid' (Krun (SState Clight.state Asm.state c2'))
                        (getCurPerm m2', snd (getThreadR Htid'))).
           (* new memory is given by the self_simulation. *)
-          exists m2', cd, f'. split; [|split; [|left]].
+          exists m2', cd, f'. repeat weak_split.
           
           + (*Reestablish the concur_match *)
             simpl.
@@ -742,7 +745,7 @@ Qed.
             exact MATCH.
           + eapply inject_incr_trace; try eassumption. 
           + (* Construct the step *)
-            exists 0%nat; simpl.
+            left; exists 0%nat; simpl.
             do 2 eexists; split; [|reflexivity].
             dilute_mem m2'.
             econstructor; eauto; simpl.
@@ -753,6 +756,7 @@ Qed.
               erewrite restr_proof_irr.
               econstructor; eauto.
             * simpl; repeat (f_equal; try eapply Axioms.proof_irr).
+          + assumption.
           + erewrite restr_proof_irr.
             eassumption.
 
@@ -794,7 +798,8 @@ Qed.
                                           U tr2 st2 m2
                                           (HybridMachineSig.yield
                                              (Scheduler:=HybridMachineSig.HybridCoarseMachine.scheduler)
-                                             U) tr2 st2' m2'.
+                                             U) tr2 st2' m2'
+      /\ inject_incr mu mu'.
       Proof.
         intros.
         inv H2.
@@ -825,7 +830,8 @@ Qed.
                                            U tr2 st2 m2
                                            (HybridMachineSig.yield
                                               (Scheduler:=HybridMachineSig.HybridCoarseMachine.scheduler)
-                                                                  U) tr2 st2' m2'.
+                                              U) tr2 st2' m2' /\
+      inject_incr mu mu'.
       Proof.
         intros * Hconcur Htrace Hchs_peek Hresume.
 
@@ -890,21 +896,20 @@ Qed.
           remember 
             (updThreadC Hcnt2 (Krun (TState Clight.state Asm.state s2'))) as st2'.
           exists st2',m2,(Some cd'), mu'. 
-          split; [|split].
+          repeat weak_split.
           + !goal (concur_match _ mu' _ _ _ _).
             admit.
           + !goal (Forall2 (inject_mevent mu') tr1 tr2).
             admit.
           + (* Step *)
             !goal (HybridMachineSig.external_step _ _ _ _ _ _ _ _).
-
-            
             assert (HH: U = (HybridMachineSig.yield
                                (Scheduler:=HybridMachineSig.HybridCoarseMachine.scheduler) U))
               by reflexivity.
             rewrite HH at 2.
             eapply HybridMachineSig.resume_step'; eauto.
             admit.
+          + assumption.
         (* econstructor; eauto. *)
 
         - (* hb < tid *)
@@ -932,7 +937,8 @@ Qed.
             concur_match cd' mu' st1' m1' st2' m2' /\
             List.Forall2 (inject_mevent mu') tr1 tr2 /\
             machine_semantics.machine_step (HybConcSem (Some (S hb)) m) tge
-                                           U tr2 st2 m2 (HybridMachineSig.schedSkip U) tr2 st2' m2'.
+                                           U tr2 st2 m2 (HybridMachineSig.schedSkip U) tr2 st2' m2'/\
+      inject_incr mu mu'.
       Proof.
         admit. (* Easy  since there is no changes to memory. *)
       Admitted.
@@ -958,7 +964,9 @@ Qed.
             concur_match cd' mu' st1' m1' st2' m2' /\
             List.Forall2 (inject_mevent mu') tr1 tr2 /\
             machine_semantics.machine_step (HybConcSem (Some (S hb)) m) tge
-                                           U tr2 st2 m2 U tr2 st2' m2'.
+                                           U tr2 st2 m2 U tr2 st2' m2'
+      /\
+      inject_incr mu mu'.
       Proof.
         admit.
         (* Easy  since there is no changes to memory. *)
@@ -981,7 +989,8 @@ Qed.
               concur_match cd' mu' st1' m1' st2' m2' /\
               List.Forall2 (inject_mevent mu') tr1' tr2' /\
               machine_semantics.machine_step (HybConcSem (Some (S hb)) m) tge U tr2 st2 m2 U' tr2' st2'
-                                             m2'.
+                                             m2' /\
+              inject_incr mu mu'.
       Proof.
         intros; simpl in H. 
         inversion H; subst.
@@ -1029,18 +1038,19 @@ Qed.
         + admit. (*should follow from compiler simulation*)
       Admitted.
 
-      
       Lemma compile_one_thread:
-        forall m,
-          HybridMachine_simulation_properties
+        forall m ,
+          simulation_properties_exposed
             (HybConcSem (Some hb) m)
             (HybConcSem (Some (S hb)) m)
             invariant
             mem_compatible
-            (concur_match).
+            (concur_match)
+            (opt_rel' (InjorderX compiler_sim)).
       Proof.
         intros.
-        econstructor.
+        unshelve econstructor;
+          [econstructor| reflexivity].
         - eapply option_wf.
           eapply (Injfsim_order_wfX compiler_sim). (*well_founded order*)
 
@@ -1065,609 +1075,5 @@ Qed.
       
     End CompileOneThread.
 
-    
-    Section CompileNThreads.
-      
-      Definition nth_index:= (list (option compiler_index)).
-      Definition list_lt: nth_index -> nth_index -> Prop:=
-        list_ord (opt_rel' (InjorderX compiler_sim)).
-
-      Lemma list_lt_wf: well_founded list_lt.
-      Proof. eapply list_ord_wf, option_wf, Injfsim_order_wfX. Qed.
-      
-      Inductive match_state:
-        forall n, nth_index ->
-          Values.Val.meminj ->
-          ThreadPool (Some 0)%nat -> Memory.Mem.mem -> ThreadPool (Some n) -> Memory.Mem.mem -> Prop:=
-      | refl_match: forall tp m,
-          (* mem_compatible tp m -> *)
-          match_state 0 nil (Mem.flat_inj (Mem.nextblock m)) tp m tp m
-      | step_match_state:
-          forall n ocd ils jn jSn tp0 m0 tpn mn tpSn mSn,
-            match_state n ils jn tp0 m0 tpn mn ->
-            concur_match n ocd jSn tpn mn tpSn mSn ->
-            match_state (S n) (cons ocd ils) (compose_meminj jn jSn) tp0 m0 tpSn mSn.
-      Lemma thread_step_mem_fwd:
-        forall hb m sge U st1 m1 st1' m1',
-          machine_semantics.thread_step (HybConcSem hb m) sge U st1 m1 st1' m1' ->
-          ((Mem.nextblock m1) <= (Mem.nextblock m1'))%positive.
-      Proof.
-        intros.
-        inv H; simpl in *.
-        inv Htstep.
-        eapply event_semantics.event_semantics_mem_fw in Hcorestep.
-        simpl in Hcorestep; auto.
-      Qed.
-      Lemma machine_step_mem_fwd:
-        forall hb m sge U tr1 st1 m1 U' tr1' st1' m1',
-          machine_semantics.machine_step (HybConcSem hb m)
-                                         sge U tr1 st1 m1 U' tr1' st1' m1'->
-          ((Mem.nextblock m1) <= (Mem.nextblock m1'))%positive.
-      Proof. Admitted.
-      
-      Lemma machine_step_trace_wf:
-        forall hb m sge U tr1 st1 m1 U' x st1' m1',
-          machine_semantics.machine_step (HybConcSem hb m)
-                                         sge U tr1 st1 m1 U' (tr1++x) st1' m1'->
-          Forall2 (inject_mevent (Mem.flat_inj (Mem.nextblock m1'))) x x.
-      Proof.
-      Admitted. (*This comes from self injection? *)
-
-      (*This should probably go soewhere else? *)
-      Lemma flat_inj_lt:
-        forall b b', (b <= b')%positive ->
-                inject_incr (Mem.flat_inj b) (Mem.flat_inj b').
-      Proof.
-        unfold Mem.flat_inj.
-        intros ** ??? HH.
-        match_case in HH. rewrite <- HH.
-        match_case.
-        xomega.
-      Qed.
-     
-      Local Ltac inv_match0:=
-        match goal with
-              H: match_state 0 _ _ _ _ _ _ |- _ =>
-              inversion H; subst_sig; try clear H
-        end.
-      Lemma Forall_cat:
-        forall {A B} (f: A -> B -> Prop) a1 a2 b1 b2,
-          Forall2 f a1 b1 ->
-          Forall2 f a2 b2 ->
-          Forall2 f (a1 ++  a2) (b1 ++ b2).
-      Proof.
-        intros A B f a1.
-        induction a1.
-        - intros. inv H.
-          do 2 rewrite seq.cat0s; auto.
-        - simpl; intros.
-          inv H. econstructor; auto.
-      Qed.
-      Lemma machine_step_traces:
-        forall hb m sge U tr1 st1 m1 U' tr1' st1' m1',
-          machine_semantics.machine_step (HybConcSem hb m)
-            sge U tr1 st1 m1 U' tr1' st1' m1'->
-          exists tr_tail, tr1' = tr1 ++ tr_tail /\
-                     forall tr2, machine_semantics.machine_step (HybConcSem hb m)
-                         sge U tr2 st1 m1 U' (tr2 ++ tr_tail) st1' m1'.
-      Admitted.
-      Lemma trivial_self_injection:
-        forall m : option mem,
-          HybridMachine_simulation_properties
-            (HybConcSem (Some 0)%nat m)
-            (HybConcSem (Some 0)%nat m)
-            invariant
-            mem_compatible
-            (match_state 0).
-      Proof.
-        simpl; intros.
-        econstructor.
-        - eapply list_lt_wf.
-        - intros; normal; eauto.
-          + econstructor.
-        - intros; normal.
-          + econstructor.
-          + eapply inject_incr_trace; try eassumption.
-            inv_match0; eapply flat_inj_lt.
-            eapply thread_step_mem_fwd; apply H.
-          + left. exists 0%nat; inv_match0.
-            do 2 eexists; split; try reflexivity; eauto.
-        - intros; inv_match0.
-          eapply machine_step_traces in H; normal; subst; eauto.
-          + econstructor.
-          + eapply Forall_cat.
-            eapply inject_incr_trace; try eassumption.
-            apply flat_inj_lt.
-            eapply machine_step_mem_fwd; eauto.
-            eapply machine_step_trace_wf; eapply H2.
-          + eapply H2.
-        - intros; inv_match0; normal; eauto.
-        - intros; inv_match0; reflexivity. 
-          Unshelve.
-          all: eauto.
-      Qed.
-      
-      
-      Lemma step_diagram_helper:
-        forall (ord: relation nth_index) tr1 tr2 m U hb cd m1' st1' tge st2 m2, 
-          (exists (st2' : ThreadPool (Some hb)) (m2' : mem) (cd' : nth_index) 
-             (mu' : meminj),
-              match_state hb cd' mu' st1' m1' st2' m2' /\
-              Forall2 (inject_mevent mu') tr1 tr2 /\
-              (machine_semantics_lemmas.thread_step_plus
-                 (HybConcSem (Some hb) m) 
-                 tge U st2 m2 st2' m2' \/
-               machine_semantics_lemmas.thread_step_star
-                 (HybConcSem (Some hb) m) 
-                 tge U st2 m2 st2' m2' /\ ord cd' cd))
-          <->
-          exists (st2' : ThreadPool (Some hb)) (m2' : mem) (cd' : nth_index) 
-            (mu' : meminj),
-            match_state hb cd' mu' st1' m1' st2' m2' /\
-            Forall2 (inject_mevent mu') tr1 tr2 /\
-            (machine_semantics_lemmas.thread_step_plus
-               (HybConcSem (Some hb) m) 
-               tge U st2 m2 st2' m2' \/  m2=m2' /\ st2=st2' /\ ord cd' cd).
-      Proof.
-        intros.
-        split; intros; normal; eauto.
-        - destruct H1; auto.
-          destruct H1 as [[n H1] Hord]; destruct n.
-          + inv H1; auto.
-          + left; exists n; auto.
-        - destruct H1; [left| right]; auto.
-          normal; subst; auto.
-          exists 0%nat. constructor.
-      Qed.
-      
-      Lemma inject_mem_event_interpolation:
-            forall jn jSn ev1 ev3,
-            (inject_mem_event (compose_meminj jn jSn)) ev1 ev3 ->
-            exists ev2,
-              inject_mem_event jn ev1 ev2 /\
-              inject_mem_event jSn ev2 ev3 .
-          Proof.
-            intros.
-            destruct ev1.
-            - inv H.
-          Admitted.
-          Lemma inject_mem_sync_interpolation:
-            forall jn jSn ev1 ev3,
-            (inject_sync_event (compose_meminj jn jSn)) ev1 ev3 ->
-            exists ev2,
-              inject_sync_event jn ev1 ev2 /\
-              inject_sync_event jSn ev2 ev3 .
-          Proof.
-            intros.
-            destruct ev1.
-            - inv H.
-          Admitted.
-          Lemma inject_mevent_interpolation:
-            forall jn jSn ev1 ev3,
-            (inject_mevent (compose_meminj jn jSn)) ev1 ev3 ->
-            exists ev2,
-              inject_mevent jn ev1 ev2 /\
-              inject_mevent jSn ev2 ev3 .
-          Proof.
-            intros.
-            destruct ev1.
-            - inv H.
-              eapply inject_mem_event_interpolation in H3.
-              normal_hyp; repeat (econstructor; eauto).
-            - inv H.
-              eapply inject_mem_sync_interpolation in H3.
-              normal_hyp; repeat (econstructor; eauto).
-          Qed.
-              
-          
-          Lemma list_inject_mevent_interpolation:
-            forall jn jSn tr1 tr3,
-            Forall2 (inject_mevent (compose_meminj jn jSn)) tr1 tr3 ->
-            exists tr2,
-              Forall2 (inject_mevent jn) tr1 tr2 /\
-              Forall2 (inject_mevent jSn) tr2 tr3 .
-          Proof.
-            intros ?? tr1.
-            induction tr1.
-            - intros tr3 HH; inv HH.
-              econstructor; eauto.
-            - intros tr3 HH; inv HH.
-              eapply IHtr1 in H3.
-              eapply inject_mevent_interpolation in H1.
-              normal_hyp.
-              eexists; repeat (econstructor; eauto).
-          Qed.            
-Lemma inject_mevent_compose:
-              forall j1 j2 t1 t2 t3,
-              inject_mevent j1 t1 t2->
-              inject_mevent j2 t2 t3->
-              inject_mevent (compose_meminj j1 j2) t1 t3.
-            Admitted.
-            Lemma forall_inject_mevent_compose:
-              forall j1 j2 t1 t2 t3,
-              Forall2 (inject_mevent j1) t1 t2->
-              Forall2 (inject_mevent j2) t2 t3->
-              Forall2 (inject_mevent (compose_meminj j1 j2)) t1 t3.
-            Proof.
-              intros ?? t1.
-              induction t1.
-              - intros. inv H. inv H0. constructor.
-              - intros. inv H. inv H0. constructor; eauto.
-                eapply inject_mevent_compose; eauto.
-            Qed.
-      Lemma simulation_inductive_case:
-        forall n : nat,
-          (forall m : option mem,
-              HybridMachine_simulation_properties
-                (HybConcSem (Some 0)%nat m)
-                (HybConcSem (Some n) m)
-                invariant
-                mem_compatible
-                (match_state n)) ->
-          (forall m : option mem,
-              HybridMachine_simulation_properties
-                (HybConcSem (Some n) m)
-                (HybConcSem (Some (S n)) m)
-                invariant
-                mem_compatible
-                (concur_match n)) ->
-          forall m : option mem,
-            HybridMachine_simulation_properties
-              (HybConcSem (Some 0)%nat m)
-              (HybConcSem (Some (S n)) m)
-              invariant
-                mem_compatible
-                (match_state (S n)).
-      Proof.
-        intros n Hsim0 Hsimn m.
-        specialize (Hsim0 m).
-        specialize (Hsimn m).
-        econstructor.
-        - !goal (well_founded _).
-          eapply list_ord_part_wf.
-          eapply Hsimn.
-          eapply Hsim0.
-        - intros.
-          eapply Hsim0 in H; normal_hyp.
-          eapply Hsimn in H; eauto.
-          normal; eauto.
-          !goal(match_state _ _ _ _ _ _ _). econstructor; eauto.
-        - intros.
-          inv H0. subst_sig.
-          eapply Hsim0 in H; eauto.
-          apply step_diagram_helper in H.
-          apply step_diagram_helper.
-          normal_hyp. destruct H2.
-          + revert H H0.
-            admit.
-          + normal_hyp; subst.
-            assert (Forall2 (inject_mevent (compose_meminj x2 jSn)) tr1 tr2).
-            { admit. (*Need an inject_incr or something about x2. *)
-            }
-            clear H1.
-            normal_goal; eauto.
-            * econstructor; eauto.
-            * right; repeat weak_split auto.
-              constructor; auto.
-        - intros.
-          inv H2; subst_sig.
-          eapply list_inject_mevent_interpolation in H3; normal_hyp.
-          eapply Hsim0 in H.
-          normal_hyp.
-          eapply Hsimn in H5; eauto.
-          normal.
-          + econstructor; eauto.
-          + instantiate(1:= x5).
-            eapply forall_inject_mevent_compose; eauto.
-          + auto.
-          + (* add match_state _ st1 m1 st2 m2 -> invariant st2 *)
-            admit.
-          + (* add match_state _ st1 m1 st2 m2 -> mem_compat st2 m2 *)
-            admit.
-          + eauto.
-          + eauto.
-          + eauto.
-          + eauto.
-        - econstructor; simpl in *.
-          unfold HybridMachineSig.halted_machine in *; simpl in *.
-          match_case in H0.
-       (* - intros * Hmatch i. inv Hmatch.
-          (eapply thread_running with (i:=i) in Hsimn); eauto. 
-          (eapply thread_running with (i:=i)  in Hsim0); eauto.
-          split; intros HH; eauto.
-          + eapply Hsimn; eapply Hsim0; assumption.
-          + eapply Hsim0; eapply Hsimn; assumption. *)
-
-            Unshelve.
-            all: assumption.
-      Admitted.
-
-      
-      Context (Hexterns_have_events: Asm_externals_have_events Asm_g).
-      Lemma compile_n_threads:
-        forall n m,
-          HybridMachine_simulation.HybridMachine_simulation_properties
-            (HybConcSem (Some 0)%nat m)
-            (HybConcSem (Some n) m)
-            invariant
-            mem_compatible
-            (match_state n).
-      Proof.
-        induction n.
-        - (*trivial reflexive induction*)
-          apply trivial_self_injection.
-        - eapply simulation_inductive_case; eauto.
-          eapply compile_one_thread; auto.
-      Qed.
-
-    End CompileNThreads.
-
-    Section CompileInftyThread.
-      Context {Hasm_externals: Asm_externals_have_events Asm_g}.
-      
-      Definition lift_state': forall {on on'},
-         ThreadPool on -> ThreadPool on'.
-      Proof.
-        intros; inv X; econstructor; eauto.
-      Defined.
-                                   
-      Inductive lift_state: forall on, ThreadPool on -> forall on', ThreadPool on' -> Prop:=
-      | build_lift_state: forall on on' st st',
-          st' = lift_state' st ->
-          lift_state on st on' st'.
-      
-      Lemma lift_invariant:
-        forall hb1 hb2 st st',
-          lift_state hb1 st hb2 st' ->
-          invariant st ->
-          invariant st'.
-      Admitted.
-      Lemma cmpt_invariant:
-        forall hb1 hb2 st st' m,
-          lift_state hb1 st hb2 st' ->
-          mem_compatible st m ->
-          mem_compatible st' m.
-      Admitted.
-
-      
-      Inductive infty_match:
-        nth_index -> meminj ->
-        ThreadPool (Some 0)%nat -> mem ->
-        ThreadPool None -> mem -> Prop:=
-      | Build_infty_match:
-          forall n cd j st0 m0 stn mn st,
-            match_state n cd j st0 m0 stn mn ->
-            lift_state (Some n) stn None st ->
-            infty_match cd j st0 m0 st mn.
-
-
-      Lemma initial_infty:
-        forall (m : option mem) (s_mem s_mem' : mem) 
-          (main : val) (main_args : list val)
-          (s_mach_state : ThreadPool (Some 0)%nat) (r1 : option res),
-          machine_semantics.initial_machine (HybConcSem (Some 0)%nat m) r1
-                                            s_mem s_mach_state s_mem' main main_args ->
-          exists
-            (j : meminj) (cd : nth_index) (t_mach_state : ThreadPool None) 
-            (t_mem t_mem' : mem) (r2 : option res),
-            machine_semantics.initial_machine (HybConcSem None m) r2 t_mem
-                                              t_mach_state t_mem' main main_args /\
-            infty_match cd j s_mach_state s_mem' t_mach_state t_mem'.
-      Proof.
-      (* Follows from any initial diagram and a missing lemma showing that the initial state
-        can be "lifted" (lift_state) *)
-      Admitted.
-
-      Lemma infinite_step_diagram:
-        forall (m : option mem) (sge tge : HybridMachineSig.G)
-          (U : list nat) tr1 (st1 : ThreadPool (Some 0)%nat) 
-          (m1 : mem) (st1' : ThreadPool (Some 0)%nat) 
-          (m1' : mem),
-          machine_semantics.thread_step (HybConcSem (Some 0)%nat m) sge U st1
-                                        m1 st1' m1' ->
-          forall (cd : nth_index) tr2 (st2 : ThreadPool None) 
-            (mu : meminj) (m2 : mem),
-            infty_match cd mu st1 m1 st2 m2 ->
-            List.Forall2 (inject_mevent mu) tr1 tr2 ->
-            exists
-              (st2' : ThreadPool None) (m2' : mem) (cd' : nth_index) 
-              (mu' : meminj),
-              infty_match cd' mu' st1' m1' st2' m2' /\
-              List.Forall2 (inject_mevent mu') tr1 tr2 /\
-              (machine_semantics_lemmas.thread_step_plus 
-                 (HybConcSem None m) tge U st2 m2 st2' m2' \/
-               machine_semantics_lemmas.thread_step_star 
-                 (HybConcSem None m) tge U st2 m2 st2' m2' /\ 
-               list_lt cd' cd).
-      Proof.
-      (*Proof sketch:
-            infty_match defines an intermediate machine Mn at level n, matching the 0 machine.
-            All threads of machine Mn are in Asm. A lemma should show that all hier machines 
-            (Mk, for k>n) also match the machine at 0. 
-            lemma [compile_n_threads] shows that machine M(S n) can step and reestablish 
-            [match_states]. Since we increased the hybrid bound (n -> S n) then the new thread 
-            is in Asm and [match_states] can be lifted to [infty_match].
-       *)
-      Admitted.
-      Lemma infinite_machine_step_diagram:
-        forall (m : option mem) (sge tge : HybridMachineSig.G)
-          (U : list nat) (tr1 : HybridMachineSig.event_trace)
-          (st1 : ThreadPool (Some 0)%nat) (m1 : mem) (U' : list nat)
-          (tr1' : HybridMachineSig.event_trace)
-          (st1' : ThreadPool (Some 0)%nat) (m1' : mem),
-          machine_semantics.machine_step (HybConcSem (Some 0)%nat m) sge U tr1
-                                         st1 m1 U' tr1' st1' m1' ->
-          
-          forall (cd : nth_index) tr2 (st2 : ThreadPool None) 
-            (mu : meminj) (m2 : mem)
-            (Hinv1': invariant st1')
-            (Hcmpt1': mem_compatible st1' m1'),
-            infty_match cd mu st1 m1 st2 m2 ->
-            List.Forall2 (inject_mevent mu) tr1 tr2 ->
-            exists
-              tr2' (st2' : ThreadPool None) (m2' : mem) (cd' : nth_index) 
-              (mu' : meminj),
-              infty_match cd' mu' st1' m1' st2' m2' /\
-              List.Forall2 (inject_mevent mu') tr1' tr2' /\
-              machine_semantics.machine_step (HybConcSem None m) tge U tr2 st2
-                                             m2 U' tr2' st2' m2'.
-      Proof.
-        intros. inv H0.
-        pose proof (compile_n_threads Hasm_externals n m) as HH.
-        eapply machine_diagram in HH; eauto.
-        normal_hyp.
-        normal; eauto.
-        - econstructor; eauto. econstructor; eauto.
-        - 
-        
-        (* Same as the other step diagram.*)
-      Admitted.
-
-      Lemma infinite_halted:
-        forall (m : option mem) (cd : nth_index) (mu : meminj)
-          (U : list nat) (c1 : ThreadPool (Some 0)%nat) 
-          (m1 : mem) (c2 : ThreadPool None) (m2 : mem) 
-          (v1 : val),
-          infty_match cd mu c1 m1 c2 m2 ->
-          machine_semantics.conc_halted (HybConcSem (Some 0)%nat m) U c1 =
-          Some v1 ->
-          exists v2 : val,
-            machine_semantics.conc_halted (HybConcSem None m) U c2 =
-            Some v2.
-      Proof.
-        intros. inv H.
-        exploit thread_halted; eauto.
-        eapply compile_n_threads, Hasm_externals.
-      Qed.
-Lemma lift_contains:
-            forall {on on'} st j,
-              ThreadPool.containsThread st j <->
-              ThreadPool.containsThread (@lift_state' on on' st) j.
-          Proof.
-            intros. simpl.
-            unfold OrdinalPool.containsThread; simpl.
-            destruct st; simpl. reflexivity.
-          Qed.
-          Lemma lift_unique_Krun:
-            forall {on on'} st i,
-              HybridMachineSig.unique_Krun st i <->
-              HybridMachineSig.unique_Krun (@lift_state' on on' st) i.
-          Proof.
-            intros; split; intros ** ? **.
-            - unshelve eapply H; eauto.
-              eapply (@lift_contains on on' st j); auto.
-              simpl. match_case; simpl.
-              clear - H0.
-              destruct st; simpl in *.
-              replace (c0 cnti) with cnti by apply Axioms.proof_irr.
-              rewrite H0.
-              reflexivity.
-            - unshelve eapply H; eauto.
-              eapply (@lift_contains on on' st j); auto.
-              simpl. match_case; simpl.
-              clear - H0.
-              destruct st; simpl in *.
-              replace (c cnti) with (cnti) by apply Axioms.proof_irr.
-              rewrite H0.
-              reflexivity.
-          Qed.
-      Lemma infinite_running:
-        forall (m : option mem) (cd : nth_index) (mu : meminj)
-          (c1 : ThreadPool (Some 0)%nat) (m1 : mem) (c2 : ThreadPool None)
-          (m2 : mem),
-          infty_match cd mu c1 m1 c2 m2 ->
-          forall i : nat,
-            machine_semantics.running_thread (HybConcSem (Some 0)%nat m) c1 i <->
-            machine_semantics.running_thread (HybConcSem None m) c2 i.
-      Proof.
-        intros. inv H.
-        inv H1.
-        subst_sig.
-        etransitivity.
-        instantiate(1:= machine_semantics.running_thread
-                          (HybConcSem (Some n%nat) m)
-                          stn i).
-        - clear H st. revert n mu cd i m c1 m1 stn m2 H0.
-          induction n.
-          + intros. inv H0. subst_sig; reflexivity.
-          + intros. inv H0. etransitivity.
-            * eapply IHn; eauto.
-            * eapply concur_match_same_running; eauto.
-        - eauto; subst_sig.
-          simpl.
-          apply lift_unique_Krun.
-      Qed.
-      Lemma compile_all_threads':
-        forall m,
-          HybridMachine_simulation.HybridMachine_simulation_properties
-            (HybConcSem (Some 0)%nat m)
-            (HybConcSem None m)
-            invariant
-            mem_compatible
-            infty_match.
-      Proof.
-        intros. 
-        (*All the proofs use the following lemma*)
-        pose proof compile_n_threads as HH.
-        econstructor.
-        - eapply list_lt_wf.
-        - apply initial_infty.
-        - apply infinite_step_diagram.
-        - intros; eapply infinite_machine_step_diagram;
-            eauto.
-        - apply infinite_halted.
-        - apply infinite_running.
-      Qed.
-      
-      Lemma infty_match_invariant:
-        forall cd mu st1 m1 st2 m2,
-          infty_match cd mu st1 m1 st2 m2 ->
-          invariant st1 ->
-          invariant st2.
-      Proof.
-        intros. inv H.
-        assert (invariant stn).
-        { clear H2; revert n st1 m1 st2 m2 cd mu stn H1 H0. clear.
-          induction n; intros.
-          - inv H1; auto.
-          - inv H1; eauto. subst_sig.
-            eapply H8.
-        }
-        eapply lift_invariant; eauto.
-      Qed.
-      Lemma infty_match_cmpt:
-        forall cd mu st1 m1 st2 m2,
-          infty_match cd mu st1 m1 st2 m2 ->
-          mem_compatible st1 m1 ->
-          mem_compatible st2 m2.
-      Proof.
-        intros. inv H.
-        assert (mem_compatible stn m2).
-        { revert n  st1 m1 H0  st2 m2 cd mu stn H2 H1. clear.
-          induction n; intros.
-          - inv H1; auto.
-          - inv H1; eauto. subst_sig.
-            eapply H9.
-        }
-        eapply cmpt_invariant; eauto.
-      Qed.
-      Lemma compile_all_threads:
-        forall m,
-          HybridMachine_simulation'
-            (HybConcSem (Some 0)%nat m)
-            (HybConcSem None m)
-            invariant
-            invariant
-            mem_compatible
-            mem_compatible.
-      Proof.
-        intros. econstructor; swap 1 3; swap 2 3.
-        { eapply compile_all_threads'. }
-        - intros; eapply infty_match_invariant; eauto.
-        - intros; eapply infty_match_cmpt; eauto.
-      Qed.
-
-    End CompileInftyThread.
-    
   End ThreadedSimulation.
 End ThreadedSimulation.
